Progress...

isabelle/RGA_Relational_Rules.thy
@@ -1,5 +1,5 @@
 theory RGA_Relational_Rules
-  imports Main
+  imports Main "~~/src/HOL/Library/Product_Order"
 begin
 
 datatype 'eid operation
@@ -28,6 +28,15 @@ where
   "\<lbrakk>sibling \<D> p l; l < p\<rbrakk> \<Longrightarrow> later_sibling \<D> p l" |
   "\<lbrakk>sibling \<D> p n; sibling \<D> p l; l < n; n < p\<rbrakk> \<Longrightarrow> later_sibling_2 \<D> p l" |
   "\<lbrakk>later_sibling \<D> p n\<rbrakk> \<Longrightarrow> has_next_sibling \<D> p"
+  
+inductive_cases list_elem_ind: "list_elem xs x"
+inductive_cases has_child_ind: "has_child xs x"
+inductive_cases child_ind: "child xs x y"
+inductive_cases later_child_ind: "later_child xs x y"
+inductive_cases sibling_ind: "sibling xs x y"
+inductive_cases later_sibling_ind: "later_sibling xs x y"
+inductive_cases later_sibling_2_ind: "later_sibling_2 xs x y"  
+inductive_cases has_next_sibling_ind: "has_next_sibling xs x"
 
 inductive first_child  :: "'eid::{linorder} database \<Rightarrow> 'eid \<Rightarrow> 'eid \<Rightarrow> bool"
   and next_sibling     :: "'eid::{linorder} database \<Rightarrow> 'eid \<Rightarrow> 'eid \<Rightarrow> bool"
@@ -41,19 +50,21 @@ where
   "\<lbrakk>first_child \<D> p n\<rbrakk> \<Longrightarrow> next_elem \<D> p n" |
   "\<lbrakk>list_elem \<D> p; \<not> has_child \<D> p; next_sibling_anc \<D> p n\<rbrakk> \<Longrightarrow> next_elem \<D> p n"  
 
+inductive_cases first_child_ind: "first_child xs x y"
+inductive_cases next_sibling_ind: "next_sibling \<D> s n"
+inductive_cases next_sibling_anc_ind: "next_sibling_anc \<D> s n"
+inductive_cases next_elem_ind: "next_elem xs x y"
+  
 lemmas rga_intros [intro] =
   list_elem_has_child_child_later_child_sibling_later_sibling_later_sibling_2_has_next_sibling.intros
   first_child_next_sibling_next_sibling_anc_next_elem.intros
-
+  
+lemmas rga_elims = list_elem_ind has_child_ind child_ind later_child_ind sibling_ind
+  later_sibling_ind later_sibling_2_ind has_next_sibling_ind first_child_ind next_sibling_ind
+  next_sibling_anc_ind next_elem_ind
+  
 definition next_elem_rel :: "'eid::{linorder} database \<Rightarrow> ('eid \<times> 'eid) set" where
   "next_elem_rel \<D> \<equiv> {(x, y). next_elem \<D> x y}"
-  
-lemma insert_serial:
-  assumes "\<D> y = None" and "\<D>' = \<D>(y \<mapsto> Insert x)"
-    and "(x, z) \<in> next_elem_rel \<D>"
-    and "\<forall>n \<in> dom \<D>. n < y"
-  shows "next_elem_rel \<D>' = next_elem_rel \<D> - {(x, z)} \<union> {(x, y), (y, z)}"
-  oops
 
 inductive list_suffix :: "'eid::{linorder} database \<Rightarrow> 'eid \<Rightarrow> 'eid list \<Rightarrow> bool"
   and list_full       :: "'eid::{linorder} database \<Rightarrow> 'eid \<Rightarrow> 'eid list \<Rightarrow> bool"
@@ -83,9 +94,6 @@ lemma parent_unique:
   and "child \<D> par2 n"
   shows "par1 = par2"
   by(metis (no_types, lifting) insert_def assms child.cases operation.inject option.inject)
-    
-inductive_cases next_sibling_ind: "next_sibling \<D> s n"
-inductive_cases next_sibling_anc_ind: "next_sibling_anc \<D> s n"
   
 lemma next_elem_unique:
   shows "first_child \<D> parent child1 \<Longrightarrow> first_child \<D> parent child2 \<Longrightarrow> child1 = child2"
@@ -101,14 +109,218 @@ lemma next_elem_unique:
     apply (metis has_next_sibling.simps next_sibling_anc.simps next_sibling_ind parent_unique)
     apply (meson child.cases first_child.cases next_elem.cases rga_intros(2))
     by (meson child.cases first_child.cases list_elem_has_child_child_later_child_sibling_later_sibling_later_sibling_2_has_next_sibling.intros(2) next_elem.cases)
-    
-    
-    
 
-lemma elem_index_biject:
-  assumes "elem_index \<D> x i" and "elem_index \<D> y j"
-  shows "i = j \<longleftrightarrow> x = y"
-  oops
+definition next_elem_fun :: "'a::{linorder} database \<Rightarrow> 'a \<Rightarrow> 'a option" where
+  "next_elem_fun \<D> prev \<equiv>
+     if \<exists>x. next_elem \<D> prev x then
+       Some (THE x. next_elem \<D> prev x)
+     else None"
+  
+definition list_of_database :: "'a::{linorder} database \<Rightarrow> ('a \<times> 'a operation) list" where
+  "list_of_database \<D> \<equiv>
+    let ss = sorted_list_of_set (dom \<D>) in
+      List.map (\<lambda>x. (x, Option.the (\<D> x))) ss"
+  
+lemma
+  assumes "list_of_database \<D> = xs"
+  shows "\<D> = map_of xs"
+  using assms
+  apply(induction xs)
+   apply(clarsimp simp add: list_of_database_def)
+  sorry
+  
+lemma not_child_empty [simp]:
+  shows "\<not> child Map.empty x y"
+  apply(clarsimp)
+  apply(erule child_ind, auto simp add: insert_def)
+  done
+    
+lemma not_first_child_empty [simp]:
+  shows "\<not> first_child Map.empty x y"
+    apply clarsimp
+  apply(erule first_child_ind)
+  apply auto
+  done
+    
+lemma not_next_sibling_anc_empty [simp]:
+  shows "\<not> next_sibling_anc Map.empty x y"
+  apply clarsimp
+  apply(erule next_sibling_anc_ind)
+   apply(erule next_sibling_ind)
+   apply(erule later_sibling_ind)
+   apply(erule sibling_ind)
+   apply simp+
+  done
+    
+lemma not_next_elem_empty [simp]:
+  shows "\<not> next_elem Map.empty x y"
+  apply clarsimp
+  apply(erule next_elem_ind)
+   apply simp+
+  done
 
+(*    
+lemma insert_serial:       
+  assumes "(x, z) \<in> next_elem_rel (map_of xs)"
+  shows "next_elem_rel (map_of (xs@[(y, Insert x)])) = next_elem_rel (map_of xs) - {(x, z)} \<union> {(x, y), (y, z)}"
+  apply(induction xs rule: List.rev_induct)
+   apply(clarsimp simp add: next_elem_rel_def)
+   apply(rule equalityI, rule subsetI, clarsimp)
+    apply(case_tac "a=y"; clarsimp)
+    apply(erule rga_elims)+
+      apply(clarsimp simp add: insert_def)
+      apply(case_tac "b=y"; clarsimp)
+     apply(erule rga_elims)+
+      apply(clarsimp simp add: insert_def)
+      apply(case_tac "b=y"; clarsimp)
+     apply(erule child_ind, clarsimp simp add: insert_def)
+     apply(erule rga_elims)+
+          apply(clarsimp simp add: insert_def)
+      apply(case_tac "b=y"; clarsimp)
+      apply force
+  
+lemma
+  assumes "list_of_database \<D> = xs @ [x] @ ys"
+    and "\<D>(fst y) = None"
+    and "\<D>' = \<D>(fst y \<mapsto> Insert (fst x))"
+    and "list_of_database \<D>' = xs @ [x] @ ys @ [y]"
+    shows "next_elem_rel \<D>' = next_elem_rel \<D> - {(x, z)} \<union> {(x, y), (y, z)}"
+  using assms
+  apply clarsimp
+  apply(induction ys rule: List.rev_induct)
+*)
+  
+    (*
+lemma
+  shows "next_elem D' a b \<Longrightarrow> D' = (\<D>(y \<mapsto> Insert x)) \<Longrightarrow> \<D> y = None \<Longrightarrow> next_elem \<D> x z \<Longrightarrow> (\<And>n. n \<in> dom \<D> \<Longrightarrow> n < y) \<Longrightarrow> a = x \<longrightarrow> b \<noteq> y \<Longrightarrow> next_elem \<D> a b \<longrightarrow> a = x \<and> b = z \<Longrightarrow> a = y \<and> b = z"
+  apply(induction rule: first_child_next_sibling_next_sibling_anc_next_elem.inducts(4))
+       prefer 5
+       apply(erule rga_elims)+
+    apply(clarsimp simp add: insert_def split: if_split_asm)
+*)
+    
+lemma child_D_None_contr:
+  assumes "D y = None"
+  shows "\<not> child D p y"
+  using assms
+  apply clarsimp
+  apply(erule child_ind)
+  apply(clarsimp simp add: insert_def)
+  done
+    
+lemma child_D_dom:
+  assumes "child D p y"
+  shows "y \<in> dom D"
+using child_D_None_contr assms by blast
+
+  (*
+list_elem    :: "'eid::{linorder} database \<Rightarrow> 'eid \<Rightarrow> bool"
+  and has_child        :: "'eid::{linorder} database \<Rightarrow> 'eid \<Rightarrow> bool"
+  and child            :: "'eid::{linorder} database \<Rightarrow> 'eid \<Rightarrow> 'eid \<Rightarrow> bool"
+  and later_child      :: "'eid::{linorder} database \<Rightarrow> 'eid \<Rightarrow> 'eid \<Rightarrow> bool"
+  and sibling          :: "'eid::{linorder} database \<Rightarrow> 'eid \<Rightarrow> 'eid \<Rightarrow> bool"
+  and later_sibling    :: "'eid::{linorder} database \<Rightarrow> 'eid \<Rightarrow> 'eid \<Rightarrow> bool"
+  and later_sibling_2  :: "'eid::{linorder} database \<Rightarrow> 'eid \<Rightarrow> 'eid \<Rightarrow> bool"
+  and has_next_sibling :: "'eid::{linorder} database \<Rightarrow> 'eid \<Rightarrow> bool"
+where
+*)
+  
+lemma later_sibling_insert_invariant_1:
+  shows "list_elem D n \<Longrightarrow> D y = None \<Longrightarrow> D' = D(y \<mapsto> Insert z) \<Longrightarrow> list_elem D' n"
+    and "has_child D n \<Longrightarrow> D y = None \<Longrightarrow> D' = D(y \<mapsto> Insert z) \<Longrightarrow> has_child D' n"
+    and "child D p n \<Longrightarrow> D y = None \<Longrightarrow> D' = D(y \<mapsto> Insert z) \<Longrightarrow> child D' p n"
+    and "later_child D p n \<Longrightarrow> D y = None \<Longrightarrow> D' = D(y \<mapsto> Insert z) \<Longrightarrow> later_child D' p n"
+    and "sibling D p n \<Longrightarrow> D y = None \<Longrightarrow> D' = D(y \<mapsto> Insert z) \<Longrightarrow>  sibling D' p n"
+    and "later_sibling D p n \<Longrightarrow> D y = None \<Longrightarrow> D' = D(y \<mapsto> Insert z) \<Longrightarrow> later_sibling D' p n"
+    and "later_sibling_2 D p n \<Longrightarrow> D y = None \<Longrightarrow> D' = D(y \<mapsto> Insert z) \<Longrightarrow> later_sibling_2 D' p n"
+    and "has_next_sibling D p \<Longrightarrow> D y = None \<Longrightarrow> D' = D(y \<mapsto> Insert z) \<Longrightarrow> has_next_sibling D' p"
+         apply(induction rule: list_elem_has_child_child_later_child_sibling_later_sibling_later_sibling_2_has_next_sibling.inducts)
+         apply(clarsimp simp add: insert_def)
+         apply(rule_tac parent=parent in rga_intros(1))
+         apply(clarsimp simp add: insert_def)
+             apply(rule_tac c=c in rga_intros(2))
+        apply(clarsimp simp add: insert_def)
+       apply(rule rga_intros)
+       apply(clarsimp simp add: insert_def)
+      apply(rule_tac p=p in rga_intros(4))
+        apply force
+       apply force
+      apply assumption
+     apply(rule_tac parent=parent in rga_intros(5))
+      apply force
+     apply force
+    apply(rule rga_intros)
+     apply force
+    apply assumption
+   apply(rule_tac n=n in rga_intros(7))
+      apply force
+     apply force
+    apply assumption
+   apply assumption
+  apply(rule rga_intros)
+    apply force
+  done
+    
+lemma later_sibling_insert_invariant_2:
+  shows "list_elem D' n \<Longrightarrow> n \<noteq> y \<Longrightarrow> D y = None \<Longrightarrow> D' = D(y \<mapsto> Insert z) \<Longrightarrow> list_elem D n"
+    and "has_child D' n \<Longrightarrow> n \<noteq> z \<Longrightarrow> D y = None \<Longrightarrow> D' = D(y \<mapsto> Insert z) \<Longrightarrow> has_child D n"
+    and "child D' p n \<Longrightarrow> n \<noteq> y \<Longrightarrow> D y = None \<Longrightarrow> D' = D(y \<mapsto> Insert z) \<Longrightarrow> child D p n"
+    and "later_child D' p n \<Longrightarrow> n \<noteq> y \<Longrightarrow> D y = None \<Longrightarrow> D' = D(y \<mapsto> Insert z) \<Longrightarrow> (z \<noteq> p \<longrightarrow> later_child D p n \<and> z = p \<longrightarrow> True)"
+    and "sibling D' p n \<Longrightarrow> n \<noteq> y \<Longrightarrow> D y = None \<Longrightarrow> D' = D(y \<mapsto> Insert z) \<Longrightarrow>  sibling D p n"
+    and "later_sibling D' p n \<Longrightarrow> n \<noteq> y \<Longrightarrow> D y = None \<Longrightarrow> D' = D(y \<mapsto> Insert z) \<Longrightarrow> later_sibling D p n"
+    and "later_sibling_2 D' p n \<Longrightarrow> n \<noteq> y \<Longrightarrow> D y = None \<Longrightarrow> D' = D(y \<mapsto> Insert z) \<Longrightarrow> later_sibling_2 D p n"
+    and "has_next_sibling D' p \<Longrightarrow> D y = None \<Longrightarrow> D' = D(y \<mapsto> Insert z) \<Longrightarrow> has_next_sibling D p"
+         apply(induction rule: list_elem_has_child_child_later_child_sibling_later_sibling_later_sibling_2_has_next_sibling.inducts)
+         apply(clarsimp simp add: insert_def)
+         apply(rule_tac parent=parent in rga_intros(1))
+         apply(clarsimp simp add: insert_def split!: if_split_asm)
+        apply(rule_tac c=c in rga_intros(2))
+        apply(clarsimp simp add: insert_def split!: if_split_asm)
+       apply(rule rga_intros)
+       apply(clarsimp simp add: insert_def split!: if_split_asm)
+      apply(rule_tac p=p in rga_intros(4))
+        apply force
+    apply force
+    
+  
+lemma insert_serial:
+  shows "first_child \<D> x z \<Longrightarrow> (\<And>n. n \<in> dom \<D> \<Longrightarrow> n < y) \<Longrightarrow> \<D> y = None \<Longrightarrow> \<D>' = \<D>(y \<mapsto> Insert x) \<Longrightarrow> \<not> first_child \<D>' x z \<and> first_child \<D>' x y"
+    and "next_sibling \<D> x z \<Longrightarrow> \<D> y = None \<Longrightarrow> \<D>' = \<D>(y \<mapsto> Insert x) \<Longrightarrow> next_sibling \<D>' x z"
+    and "next_sibling_anc \<D> x z \<Longrightarrow> \<D> y = None \<Longrightarrow> \<D>' = \<D>(y \<mapsto> Insert x) \<Longrightarrow> next_sibling_anc \<D>' x z"
+    and "next_elem \<D> x z \<Longrightarrow> (\<And>n. n \<in> dom \<D> \<Longrightarrow> n < y) \<Longrightarrow> \<D> y = None \<Longrightarrow> \<D>' = \<D>(y \<mapsto> Insert x) \<Longrightarrow> \<not> next_elem \<D>' x z \<and> next_elem \<D>' x y \<and> next_elem \<D>' y z"
+     apply(induction rule: first_child_next_sibling_next_sibling_anc_next_elem.inducts)
+       apply clarsimp
+       apply(rule conjI, rule notI)
+  apply(erule first_child_ind)
+  apply(erule child_ind) back
+        apply(clarsimp simp add: insert_def split: if_split_asm)
+  using child_D_None_contr apply metis
+        apply(subgoal_tac "later_child (\<D>(y \<mapsto> Insert parent)) parent c", force)
+        apply(rule rga_intros(4)[where p="y"])
+          apply(rule rga_intros, clarsimp simp add: insert_def)+
+        apply force
+       apply(rule rga_intros)
+        apply(rule rga_intros, clarsimp simp add: insert_def)+
+       apply(rule notI)
+       apply(erule later_child_ind)
+       apply(subgoal_tac "p \<in> dom \<D>", force)
+  using child_D_dom apply(metis domIff fun_upd_other neq_iff)
+    apply(rule rga_intros)
+    using later_sibling_insert_invariant apply blast
+    using later_sibling_insert_invariant apply metis
+       apply(rule rga_intros)
+      using later_sibling_insert_invariant apply blast
+      defer
+       
+
+    
+lemma insert_serial:
+  assumes "\<D> y = None" and "\<D>' = \<D>(y \<mapsto> Insert x)"
+    and "(x, z) \<in> next_elem_rel \<D>"
+    and "\<And>n. n \<in> dom \<D> \<Longrightarrow> n < y"
+  shows "next_elem_rel \<D>' = next_elem_rel \<D> - {(x, z)} \<union> {(x, y), (y, z)}"
+using assms
+  apply(clarsimp simp add: next_elem_rel_def)
+  apply(rule equalityI, rule subsetI; clarsimp)
 
 end
